proof/correctness/Utils.ec
@@ -5,6 +5,14 @@ from Jasmin require import JModel.
 lemma lte_lt (a b : int) :
     a <= b => a < b \/ a = b by smt().
 
-pred valid_ptr(p : int, o : int) = 
-  0 <= o => 
-    0 <= p /\ p + o < W64.modulus.
+lemma neg_lt (x y : int) : ! (x < y) <=> y <= x by smt().
+
+lemma plus_lt (a b c : int) :
+    a + b < c <=> b < (c - a) by smt().
+
+lemma add_u (a b c : int) :
+    a + b = a + c <=> b = c by smt().
+
+pred valid_ptr(base_ptr offset : W64.t) = 
+  0 <= to_uint offset => 
+    0 <= to_uint base_ptr /\ to_uint (base_ptr + offset) < W64.modulus.
